src/StructuredEncryption/src/StructuredEncryptionConstants.dfy
@@ -1,0 +1,10 @@
+// Copyright Amazon.com Inc. or its affiliates. All Rights Reserved.
+// SPDX-License-Identifier: Apache-2.0
+include "../../../private-aws-encryption-sdk-dafny-staging/src/StandardLibrary/StandardLibrary.dfy"
+
+// TODO due to how we are building right now, we can't just name this "Constants"
+// or we run into a "duplicate module" error
+module StructuredEncryptionConstants {
+    import opened StandardLibrary.UInt
+    const BYTES_TYPE_ID : seq<uint8> := [0xFF, 0xFF];
+}
